list: prove offer & poll using known encoding

misc/list.bpl
@@ -27,13 +27,19 @@ var tail: Loc;
 function {:inline} Inv(heap: Heap, head: Loc, tail: Loc) : bool
 {
   BetweenSet(next(heap), head, null)[head] && BetweenSet(next(heap), head, null)[tail]
-    && Subset(BetweenSet(next(heap), head, null), Union(Singleton(null), dom(heap)))
+    && (forall l: Loc :: known(l) ==> (Between(next(heap), head, l, null) ==> l == null || dom(heap)[l]))
+    //    && Subset(BetweenSet(next(heap), head, null), Union(Singleton(null), dom(heap)))
+    && tail != null
+    && known(head) && known(tail) && known(null) && knownF(next(heap))
 }
 
 // ---------- Primitives/helpers for modifying global state
 
 
-procedure {:inline 1} alloc(x: Loc)
+procedure alloc(x: Loc)
+  requires !dom(heap)[x] && x != null;
+  ensures heap == Add(old(heap), x, null);
+  ensures knownF(next(heap));
   modifies heap;
 {
   assert !dom(heap)[x];
@@ -45,18 +51,56 @@ procedure {:inline 1} read_tail() returns (t: Loc)
   t := tail;
 }
 
+procedure {:inline 1} read_head() returns (h: Loc)
+{
+  h := head;
+}
+
 procedure {:inline 1} read_next(x: Loc) returns (y: Loc)
+  ensures known(y);
 {
   y := next(heap)[x];
 }
 
-procedure {:inline 2} cas_next(x, x_old, x_new: Loc)
+procedure cas_next(x, x_old, x_new: Loc)
   returns (res: bool)
+  requires dom(heap)[x];
+  ensures next(old(heap))[x] == x_old ==> res && heap == Add(old(heap), x, x_new);
+  ensures next(old(heap))[x] != x_old ==> !res && heap == old(heap);
+  ensures knownF(next(heap));
   modifies heap;
 {
   assert dom(heap)[x];
   if (next(heap)[x] == x_old) {
     heap := Add(heap, x, x_new);
+    res := true;
+  } else {
+    res := false;
+  }
+}
+
+procedure cas_tail(t_old, t_new: Loc)
+  returns (res: bool)
+  ensures old(tail) == t_old ==> res && tail == t_new;
+  ensures old(tail) != t_old ==> !res && tail == old(tail);
+  modifies tail;
+{
+  if (tail == t_old) {
+    tail := t_new;
+    res := true;
+  } else {
+    res := false;
+  }
+}
+
+procedure cas_head(h_old, h_new: Loc)
+  returns (res: bool)
+  ensures old(head) == h_old ==> res && head == h_new;
+  ensures old(head) != h_old ==> !res && head == old(head);
+  modifies head;
+{
+  if (head == h_old) {
+    head := h_new;
     res := true;
   } else {
     res := false;
@@ -70,21 +114,22 @@ procedure {:inline 2} cas_next(x, x_old, x_new: Loc)
 procedure offer(v: int, x: Loc)
   returns (res: bool)
   requires Inv(heap, head, tail);
-  // Assume x_Heap has node at location x with value v
-  //  requires dom(x_Heap)[x]; // && data(x_Heap)[x] == v;
   ensures Inv(heap, head, tail);
   modifies heap, tail;
 {
   var t, tn: Loc;
   var b: bool;
-  assume !BetweenSet(next(heap), head, null)[x] && !dom(heap)[x];
+  assume !Between(next(heap), head, x, null) && !dom(heap)[x];
 
+  assert known(x);
   assert Inv(heap, head, tail);
   call alloc(x);
   assert Inv(heap, head, tail);
 
   while (true)
     invariant Inv(heap, head, tail);
+    invariant known(x) && x != null && dom(heap)[x] && next(heap)[x] == null;
+    invariant !Between(next(heap), head, x, null);
   {
     call t := read_tail();
     assert Inv(heap, head, tail);
@@ -95,19 +140,50 @@ procedure offer(v: int, x: Loc)
       assert Inv(heap, head, tail);
       call b := cas_next(t, tn, x);
       if (b) {
-        heap := Add(heap, t, x);
+        // TODO prove that abstract state now has v in it
         res := true;
-  
+
         assert Inv(heap, head, tail);
         return;
       }
     } else {
-      // call b:= cas_tail(t, tn);
-      assume tail != null;
-      tail := tn;
-      assert BetweenSet(next(heap), head, null)[tail];
+      call b:= cas_tail(t, tn);
 
       assert Inv(heap, head, tail);
+    }
+  }
+}
+
+procedure poll()
+  returns (v: int)
+  requires Inv(heap, head, tail);
+  ensures Inv(heap, head, tail);
+  modifies heap, head, tail;
+{
+  var h, h1, t, x: Loc;
+  var b: bool;
+
+  while (true)
+    invariant Inv(heap, head, tail);
+  {
+    call h := read_head();
+    call t := read_tail();
+    call x := read_next(h);
+
+    call h1 := read_head();
+    if (h == h1) {  // TODO is this really necessary?
+      if (h == t) {
+        if (x == null) {
+          return; // Queue is empty
+        }
+        call b := cas_tail(t, x);
+      } else {
+        // TODO return value in x
+        call b := cas_head(h, x);
+        if (b) {
+          return;
+        }
+      }
     }
   }
 }
@@ -115,6 +191,13 @@ procedure offer(v: int, x: Loc)
 
 // ---------- Reachability, between, and associated theories
 
+// Predicates used to control the triggers on the below axioms
+function known(x: Loc) : bool;
+function knownF(f: [Loc]Loc) : bool;
+axiom(forall x: Loc :: {known(x)} known(x));
+axiom(forall f: [Loc]Loc :: {knownF(f)} knownF(f));
+
+ 
 function Equal([Loc]bool, [Loc]bool) returns (bool);
 function Subset([Loc]bool, [Loc]bool) returns (bool);
 
@@ -148,9 +231,9 @@ function BetweenSet(f: [Loc]Loc, x: Loc, z: Loc) returns ([Loc]bool);
 ////////////////////////////////////////////////////
 // axioms relating Between and BetweenSet
 ////////////////////////////////////////////////////
-axiom(forall f: [Loc]Loc, x: Loc, y: Loc, z: Loc :: {BetweenSet(f, x, z)[y]} BetweenSet(f, x, z)[y] <==> Between(f, x, y, z));
-axiom(forall f: [Loc]Loc, x: Loc, y: Loc, z: Loc :: {Between(f, x, y, z), BetweenSet(f, x, z)} Between(f, x, y, z) ==> BetweenSet(f, x, z)[y]);
-axiom(forall f: [Loc]Loc, x: Loc, z: Loc :: {BetweenSet(f, x, z)} Between(f, x, x, x));
+axiom(forall f: [Loc]Loc, x: Loc, y: Loc, z: Loc :: {knownF(f), known(x), known(y), known(z)} BetweenSet(f, x, z)[y] <==> Between(f, x, y, z));
+axiom(forall f: [Loc]Loc, x: Loc, y: Loc, z: Loc :: {knownF(f), known(x), known(y), known(z)} Between(f, x, y, z) ==> BetweenSet(f, x, z)[y]);
+axiom(forall f: [Loc]Loc, x: Loc :: {knownF(f), known(x)} Between(f, x, x, x));
 axiom(forall f: [Loc]Loc, x: Loc, z: Loc :: {BetweenSet(f, x, z)} Between(f, z, z, z));
 
 
@@ -162,43 +245,43 @@ axiom(forall f: [Loc]Loc, x: Loc, z: Loc :: {BetweenSet(f, x, z)} Between(f, z, 
 axiom(forall f: [Loc]Loc, x: Loc :: Between(f, x, x, x));
 
 // step
-axiom(forall f: [Loc]Loc, x: Loc, y: Loc, z: Loc, w:Loc :: {Between(f, y, z, w), f[x]} Between(f, x, f[x], f[x]));
+axiom(forall f: [Loc]Loc, x: Loc :: {f[x]} Between(f, x, f[x], f[x]));
 
 // reach
-axiom(forall f: [Loc]Loc, x: Loc, y: Loc :: {f[x], Between(f, x, y, y)} Between(f, x, y, y) ==> x == y || Between(f, x, f[x], y));
+axiom(forall f: [Loc]Loc, x: Loc, y: Loc :: {f[x], known(y)} Between(f, x, y, y) ==> x == y || Between(f, x, f[x], y));
 
 // cycle
-axiom(forall f: [Loc]Loc, x: Loc, y:Loc :: {f[x], Between(f, x, y, y)} f[x] == x && Between(f, x, y, y) ==> x == y);
+axiom(forall f: [Loc]Loc, x: Loc, y:Loc :: {f[x], known(y)} f[x] == x && Between(f, x, y, y) ==> x == y);
 
 // sandwich
-axiom(forall f: [Loc]Loc, x: Loc, y: Loc :: {Between(f, x, y, x)} Between(f, x, y, x) ==> x == y);
+axiom(forall f: [Loc]Loc, x: Loc, y: Loc :: {knownF(f), known(x), known(y)} Between(f, x, y, x) ==> x == y);
 
 // order1
-axiom(forall f: [Loc]Loc, x: Loc, y: Loc, z: Loc :: {Between(f, x, y, y), Between(f, x, z, z)} Between(f, x, y, y) && Between(f, x, z, z) ==> Between(f, x, y, z) || Between(f, x, z, y));
+axiom(forall f: [Loc]Loc, x: Loc, y: Loc, z: Loc :: {knownF(f), known(x), known(y), known(z)} Between(f, x, y, y) && Between(f, x, z, z) ==> Between(f, x, y, z) || Between(f, x, z, y));
 
 // order2
-axiom(forall f: [Loc]Loc, x: Loc, y: Loc, z: Loc :: {Between(f, x, y, z)} Between(f, x, y, z) ==> Between(f, x, y, y) && Between(f, y, z, z));
+axiom(forall f: [Loc]Loc, x: Loc, y: Loc, z: Loc :: {knownF(f), known(x), known(y), known(z)} Between(f, x, y, z) ==> Between(f, x, y, y) && Between(f, y, z, z));
 
 // transitive1
-axiom(forall f: [Loc]Loc, x: Loc, y: Loc, z: Loc :: {Between(f, x, y, y), Between(f, y, z, z)} Between(f, x, y, y) && Between(f, y, z, z) ==> Between(f, x, z, z));
+axiom(forall f: [Loc]Loc, x: Loc, y: Loc, z: Loc :: {knownF(f), known(x), known(y), known(z)} Between(f, x, y, y) && Between(f, y, z, z) ==> Between(f, x, z, z));
 
 // transitive2
-axiom(forall f: [Loc]Loc, x: Loc, y: Loc, z: Loc, w: Loc :: {Between(f, x, y, z), Between(f, y, w, z)} Between(f, x, y, z) && Between(f, y, w, z) ==> Between(f, x, y, w) && Between(f, x, w, z));
+axiom(forall f: [Loc]Loc, x: Loc, y: Loc, z: Loc, w: Loc :: {knownF(f), known(x), known(y), known(z), known(w)} Between(f, x, y, z) && Between(f, y, w, z) ==> Between(f, x, y, w) && Between(f, x, w, z));
 
 // transitive3
-axiom(forall f: [Loc]Loc, x: Loc, y: Loc, z: Loc, w: Loc :: {Between(f, x, y, z), Between(f, x, w, y)} Between(f, x, y, z) && Between(f, x, w, y) ==> Between(f, x, w, z) && Between(f, w, y, z));
+axiom(forall f: [Loc]Loc, x: Loc, y: Loc, z: Loc, w: Loc :: {knownF(f), known(x), known(y), known(z), known(w)} Between(f, x, y, z) && Between(f, x, w, y) ==> Between(f, x, w, z) && Between(f, w, y, z));
 
 // This axiom is required to deal with the incompleteness of the trigger for the reflexive axiom.
 // It cannot be proved using the rest of the axioms.
-axiom(forall f: [Loc]Loc, u:Loc, x: Loc :: {Between(f, u, x, x)} Between(f, u, x, x) ==> Between(f, u, u, x));
+axiom(forall f: [Loc]Loc, u:Loc, x: Loc :: {knownF(f), known(x), known(u)} Between(f, u, x, x) ==> Between(f, u, u, x));
 
 // relation between Avoiding and Between
-axiom(forall f: [Loc]Loc, x: Loc, y: Loc, z: Loc :: {Avoiding(f, x, y, z)} Avoiding(f, x, y, z) <==> (Between(f, x, y, z) || (Between(f, x, y, y) && !Between(f, x, z, z))));
-axiom(forall f: [Loc]Loc, x: Loc, y: Loc, z: Loc :: {Between(f, x, y, z)} Between(f, x, y, z) <==> (Avoiding(f, x, y, z) && Avoiding(f, x, z, z)));
+axiom(forall f: [Loc]Loc, x: Loc, y: Loc, z: Loc :: {knownF(f), known(x), known(y), known(z)} Avoiding(f, x, y, z) <==> (Between(f, x, y, z) || (Between(f, x, y, y) && !Between(f, x, z, z))));
+axiom(forall f: [Loc]Loc, x: Loc, y: Loc, z: Loc :: {knownF(f), known(x), known(y), known(z)} Between(f, x, y, z) <==> (Avoiding(f, x, y, z) && Avoiding(f, x, z, z)));
 
 // update
-axiom(forall f: [Loc]Loc, u: Loc, v: Loc, x: Loc, p: Loc, q: Loc :: {Avoiding(f[p := q], u, v, x)} Avoiding(f[p := q], u, v, x) <==> ((Avoiding(f, u, v, p) && Avoiding(f, u, v, x)) || (Avoiding(f, u, p, x) && p != x && Avoiding(f, q, v, p) && Avoiding(f, q, v, x))));
+axiom(forall f: [Loc]Loc, u: Loc, v: Loc, x: Loc, p: Loc, q: Loc :: {knownF(f), known(x), known(u), known(v), known(p), known(q)} Avoiding(f[p := q], u, v, x) <==> ((Avoiding(f, u, v, p) && Avoiding(f, u, v, x)) || (Avoiding(f, u, p, x) && p != x && Avoiding(f, q, v, p) && Avoiding(f, q, v, x))));
 
-axiom (forall f: [Loc]Loc, p: Loc, q: Loc, u: Loc, w: Loc :: {BetweenSet(f[p := q], u, w)} Avoiding(f, u, w, p) ==> Equal(BetweenSet(f[p := q], u, w), BetweenSet(f, u, w)));
-axiom (forall f: [Loc]Loc, p: Loc, q: Loc, u: Loc, w: Loc :: {BetweenSet(f[p := q], u, w)} p != w && Avoiding(f, u, p, w) && Avoiding(f, q, w, p) ==> Equal(BetweenSet(f[p := q], u, w), Union(BetweenSet(f, u, p), BetweenSet(f, q, w))));
-axiom (forall f: [Loc]Loc, p: Loc, q: Loc, u: Loc, w: Loc :: {BetweenSet(f[p := q], u, w)} Avoiding(f, u, w, p) || (p != w && Avoiding(f, u, p, w) && Avoiding(f, q, w, p)) || Equal(BetweenSet(f[p := q], u, w), Empty()));
+axiom (forall f: [Loc]Loc, p: Loc, q: Loc, u: Loc, w: Loc :: {knownF(f), known(p), known(q), known(u), known(w)} Avoiding(f, u, w, p) ==> Equal(BetweenSet(f[p := q], u, w), BetweenSet(f, u, w)));
+axiom (forall f: [Loc]Loc, p: Loc, q: Loc, u: Loc, w: Loc :: {knownF(f), known(p), known(q), known(u), known(w)} p != w && Avoiding(f, u, p, w) && Avoiding(f, q, w, p) ==> Equal(BetweenSet(f[p := q], u, w), Union(BetweenSet(f, u, p), BetweenSet(f, q, w))));
+axiom (forall f: [Loc]Loc, p: Loc, q: Loc, u: Loc, w: Loc :: {knownF(f), known(p), known(q), known(u), known(w)} Avoiding(f, u, w, p) || (p != w && Avoiding(f, u, p, w) && Avoiding(f, q, w, p)) || Equal(BetweenSet(f[p := q], u, w), Empty()));
